Taint analysis: Add new AES instructions

src/arch/x64/X64.Leakage_Ins_Xmm_i.fst
@@ -38,12 +38,12 @@ let check_if_pxor_leakage_free ins ts =
   if src = dst then begin
     let ts' = set_xmm_taint ts dst Public in
     Classical.forall_intro quad32_xor_lemma;
-    true, TaintState ts'.regTaint Secret Secret ts'.xmmTaint
+    true, TaintState ts'.regTaint ts.flagsTaint ts.cfFlagsTaint ts'.xmmTaint
   end 
   else begin
     let taint = merge_taint (xmm_taint ts dst) (xmm_taint ts src) in
     let ts' = set_xmm_taint ts dst taint in
-    true, TaintState ts'.regTaint Secret Secret ts'.xmmTaint
+    true, TaintState ts'.regTaint ts.flagsTaint ts.cfFlagsTaint ts'.xmmTaint
   end
 
 val check_if_paddd_leakage_free: (ins:tainted_ins{let i, _, _ = ins.ops in Paddd? i}) -> (ts:taintState) -> (res:(bool*taintState){let b, ts' = res in b2t b ==>
@@ -62,7 +62,7 @@ let check_if_pslld_leakage_free ins ts =
   let Pslld dst amt, _, _ = ins.ops in
   let taint = xmm_taint ts dst in
   let ts' = set_xmm_taint ts dst taint in
-  true, TaintState ts'.regTaint Secret Secret ts'.xmmTaint
+  true, TaintState ts'.regTaint ts.flagsTaint ts.cfFlagsTaint ts'.xmmTaint
 
 val check_if_psrld_leakage_free: (ins:tainted_ins{let i, _, _ = ins.ops in Psrld? i}) -> (ts:taintState) -> (res:(bool*taintState){let b, ts' = res in b2t b ==>
      isConstantTime (Ins ins) ts /\ isLeakageFree (Ins ins) ts ts'})
@@ -71,7 +71,7 @@ let check_if_psrld_leakage_free ins ts =
   let Psrld dst amt, _, _ = ins.ops in
   let taint = xmm_taint ts dst in
   let ts' = set_xmm_taint ts dst taint in
-  true, TaintState ts'.regTaint Secret Secret ts'.xmmTaint
+  true, TaintState ts'.regTaint ts.flagsTaint ts.cfFlagsTaint ts'.xmmTaint
 
 val check_if_pshufb_leakage_free: (ins:tainted_ins{let i, _, _ = ins.ops in Pshufb? i}) -> (ts:taintState) -> (res:(bool*taintState){let b, ts' = res in b2t b ==>
      isConstantTime (Ins ins) ts /\ isLeakageFree (Ins ins) ts ts'})
@@ -89,21 +89,80 @@ let check_if_pshufd_leakage_free ins ts =
   let Pshufd dst src _, _, _ = ins.ops in
   let taint = merge_taint (xmm_taint ts dst) (xmm_taint ts src) in
   let ts' = set_xmm_taint ts dst taint in
-  true, TaintState ts'.regTaint Secret Secret ts'.xmmTaint
+  true, TaintState ts'.regTaint ts.flagsTaint ts.cfFlagsTaint ts'.xmmTaint
+
+val check_if_pextrq_leakage_free: (ins:tainted_ins{let i, _, _ = ins.ops in Pextrq? i}) -> (ts:taintState) -> (res:(bool*taintState){let b, ts' = res in b2t b ==>
+     isConstantTime (Ins ins) ts /\ isLeakageFree (Ins ins) ts ts'})
+
+open Words.Two_s
+open Words.Four_s
+
+let check_if_pextrq_leakage_free_aux (ins:tainted_ins{let i, _, _ = ins.ops in Pextrq? i}) ts =
+  let Pextrq dst src index, _, _ = ins.ops in
+  let fixedTime = operand_does_not_use_secrets dst ts in
+  assert (fixedTime ==> isConstantTime (Ins ins) ts);
+  let taint = merge_taint (operand_taint dst ts Public) (xmm_taint ts src) in
+  let taint = merge_taint taint ins.t in
+  if OMem? dst && taint <> ins.t then false, ts
+  else
+  let ts' = set_taint dst ts taint in
+  fixedTime, TaintState ts'.regTaint ts.flagsTaint ts.cfFlagsTaint ts'.xmmTaint  
+
+val lemma_if_pextrq_leakage_free_aux: (ins:tainted_ins{let i, _, _ = ins.ops in Pextrq? i}) -> (ts:taintState) -> (s1:traceState) -> (s2:traceState) -> (fuel:nat) -> Lemma
+(let b, ts' = check_if_pextrq_leakage_free_aux ins ts in b2t b ==>
+     isConstantTime (Ins ins) ts /\ isExplicitLeakageFreeGivenStates (Ins ins) fuel ts ts' s1 s2)
+
+
+let lemma_if_pextrq_leakage_free_aux ins ts s1 s2 fuel =
+  let Pextrq dst src index, _, _ = ins.ops in
+  match dst with
+  | OConst _ -> ()
+  | OReg _ -> ()
+  | OMem m ->
+  let ptr1 = eval_maddr m s1.state in
+  let ptr2 = eval_maddr m s2.state in
+  let v1 = eval_xmm src s1.state in
+  let v2 = eval_xmm src s2.state in
+  let v1 = four_to_two_two v1 in
+  let v2 = four_to_two_two v2 in
+  let v1 = two_to_nat 32 (two_select v1 (index % 2)) in
+  let v2 = two_to_nat 32 (two_select v2 (index % 2)) in
+  lemma_store_load_mem64 ptr1 v1 s1.state.mem;
+  lemma_store_load_mem64 ptr2 v2 s2.state.mem;
+  lemma_valid_store_mem64 ptr1 v1 s1.state.mem;
+  lemma_valid_store_mem64 ptr2 v2 s2.state.mem;
+  lemma_frame_store_mem64 ptr1 v1 s1.state.mem;
+  lemma_frame_store_mem64 ptr2 v2 s2.state.mem  
+
+
+let check_if_pextrq_leakage_free ins ts =
+  Classical.forall_intro_3 (lemma_if_pextrq_leakage_free_aux ins ts);
+  check_if_pextrq_leakage_free_aux ins ts
 
 val check_if_pinsrd_leakage_free: (ins:tainted_ins{let i, _, _ = ins.ops in Pinsrd? i}) -> (ts:taintState) -> (res:(bool*taintState){let b, ts' = res in b2t b ==>
      isConstantTime (Ins ins) ts /\ isLeakageFree (Ins ins) ts ts'})
 
 let check_if_pinsrd_leakage_free ins ts =
-  false, ts
-  // let Pinsrd dst src _, _, _ = ins.ops in
-  // let fixedTime = operand_does_not_use_secrets src ts in
-  // assert (fixedTime ==> isConstantTime (Ins ins) ts);
-  // let taint = merge_taint (xmm_taint ts dst) (operand_taint src ts) in
-  // let taint = merge_taint taint ins.t in
-  // let ts' = set_xmm_taint ts dst taint in
-  // fixedTime, TaintState ts'.regTaint Secret Secret ts'.xmmTaint
+  let Pinsrd dst src i, _, _ = ins.ops in
+  let fixedTime = operand_does_not_use_secrets src ts in
+  assert (fixedTime ==> isConstantTime (Ins ins) ts);
+  let taint = merge_taint (xmm_taint ts dst) (operand_taint src ts Public) in
+  let taint = merge_taint taint ins.t in
+  let ts' = set_xmm_taint ts dst taint in
+  fixedTime, TaintState ts'.regTaint ts.flagsTaint ts.cfFlagsTaint ts'.xmmTaint
 
+val check_if_pinsrq_leakage_free: (ins:tainted_ins{let i, _, _ = ins.ops in Pinsrq? i}) -> (ts:taintState) -> (res:(bool*taintState){let b, ts' = res in b2t b ==>
+     isConstantTime (Ins ins) ts /\ isLeakageFree (Ins ins) ts ts'})
+
+let check_if_pinsrq_leakage_free ins ts =
+  let Pinsrq dst src _, _, _ = ins.ops in
+  let fixedTime = operand_does_not_use_secrets src ts in
+  assert (fixedTime ==> isConstantTime (Ins ins) ts);
+  let taint = merge_taint (xmm_taint ts dst) (operand_taint src ts Public) in
+  let taint = merge_taint taint ins.t in
+  let ts' = set_xmm_taint ts dst taint in
+  fixedTime, TaintState ts'.regTaint ts.flagsTaint ts.cfFlagsTaint ts'.xmmTaint
+  
 val check_if_vpslldq_leakage_free: (ins:tainted_ins{let i, _, _ = ins.ops in VPSLLDQ? i}) -> (ts:taintState) -> (res:(bool*taintState){let b, ts' = res in b2t b ==>
      isConstantTime (Ins ins) ts /\ isLeakageFree (Ins ins) ts ts'})
 
@@ -111,7 +170,7 @@ let check_if_vpslldq_leakage_free ins ts =
   let VPSLLDQ dst src _, _, _ = ins.ops in
   let taint = merge_taint (xmm_taint ts dst) (xmm_taint ts src) in
   let ts' = set_xmm_taint ts dst taint in
-  true, TaintState ts'.regTaint Secret Secret ts'.xmmTaint
+  true, TaintState ts'.regTaint ts.flagsTaint ts.cfFlagsTaint ts'.xmmTaint
 
 val check_if_pclmuldqd_leakage_free: (ins:tainted_ins{let i, _, _ = ins.ops in Pclmulqdq? i}) -> (ts:taintState) -> (res:(bool*taintState){let b, ts' = res in b2t b ==>
      isConstantTime (Ins ins) ts /\ isLeakageFree (Ins ins) ts ts'})
@@ -189,7 +248,9 @@ let check_if_xmm_ins_consumes_fixed_time ins ts =
     | Psrld dst amt -> check_if_psrld_leakage_free ins ts
     | Pshufb dst src -> check_if_pshufb_leakage_free ins ts
     | Pshufd dst src permutation -> check_if_pshufd_leakage_free ins ts
-    | Pinsrd dst srx index -> check_if_pinsrd_leakage_free ins ts
+    | Pinsrd _ _ _  -> check_if_pinsrd_leakage_free ins ts
+    | Pinsrq _ _ _ -> check_if_pinsrq_leakage_free ins ts
+    | Pextrq _ _ _ -> check_if_pextrq_leakage_free ins ts
     | VPSLLDQ dst src count -> check_if_vpslldq_leakage_free ins ts
     | MOVDQU dst src -> false, ts
     | Pclmulqdq dst src imm -> check_if_pclmuldqd_leakage_free ins ts
@@ -199,5 +260,4 @@ let check_if_xmm_ins_consumes_fixed_time ins ts =
     | AESNI_dec_last dst src -> check_if_aesni_dec_last_leakage_free ins ts
     | AESNI_imc dst src -> check_if_aesni_imc_leakage_free ins ts
     | AESNI_keygen_assist dst src imm -> check_if_aesni_keygen_leakage_free ins ts
-    | _ -> false, ts // Unsupported yet
     
